lean/Och/Macro.lean
@@ -39,6 +39,7 @@ declare_syntax_cat och
 
 syntax:100 ident                                    : och
 syntax:100 "Type"                                   : och
+syntax:100 "Bot"                                    : och
 syntax:100 "(" och ":" och ")"                      : och
 syntax:100 "(" och ")"                              : och
 syntax:50  och:50 och:51                            : och
@@ -70,6 +71,8 @@ partial def expand (ctx : List String) (stx : TSyntax `och) : MacroM (TSyntax `t
   match stx with
   | `(och| Type) =>
     `(Expr.type)
+  | `(och| Bot) =>
+    `(Expr.bot)
   | `(och| ($a : $b)) =>
     let a' ← expand ctx a; let b' ← expand ctx b
     `(Expr.asc $a' $b')
